template-rocq/theories/Typing.v
@@ -1403,11 +1403,13 @@ Proof.
              apply (IH (_; _; _; Hs)). }
         -- pose proof (onProjections Xg); auto.
         -- pose proof (ind_sorts Xg) as Xg'. unfold check_ind_sorts in *.
-           destruct Sort.to_family; auto.
-           split. apply Xg'. destruct indices_matter; auto.
-           eapply type_local_ctx_impl. eapply Xg'. auto. intros ?? Hj. apply Xj; tas.
-           apply lift_typing_impl with (1 := Hj); intros ?? Hs. split; tas.
-           apply (IH (_; _; _; Hs)).
+           destruct Sort.to_quality; auto; split.
+           1, 3: apply Xg'.
+           all: destruct indices_matter; auto; eapply type_local_ctx_impl.
+           1, 4: eapply Xg'.
+           1, 3: auto.
+           all: intros ?? Hj; apply Xj; tas; apply lift_typing_impl with (1 := Hj);
+             intros ?? Hs; split; tas; apply (IH (_; _; _; Hs)). 
         -- apply (ind_relevance_compat Xg).
         -- apply (onIndices Xg).
       * apply All_local_env_impl with (1 := onP); intros ?? Hj. apply Xj; tas.
